\documentclass[12pt]{article}

\usepackage[a4paper, left=2.2cm, top=1.5cm, right=2.2cm, bottom=1.5cm]{geometry}
\usepackage{times, graphicx, amsmath}
\usepackage{url, multirow, color}
\usepackage[hidelinks]{hyperref}
\usepackage[font=small,labelfont=bf]{caption}

% \usepackage{titlesec}
% \titleformat{\section}{\normalfont\Large\bfseries}{Question~\thesection}{1em}{}

\renewcommand{\floatpagefraction}{0.95}
\renewcommand{\textfraction}{0}
\renewcommand{\topfraction}{1}
\renewcommand{\bottomfraction}{1}


\begin{document}
\thispagestyle{empty}

\title{Derivation of steady-state solution for $D(x_s)$ ($n\leq 4$)}
\author{Jake Aylmer}
\maketitle

\normalsize
\noindent
The steady state solutions are given by
\begin{equation}\label{eq:steadystatesolutions}
L_nT_n + \delta_{0n}A = QH_n
\end{equation}
where $L_n = n(n+1)D+B$ and
\begin{equation}\label{eq:Hn}
H_n = H_n(x_s) = (2n+1)\int_0^1 P_n(x)a(x,x_s)S(x)dx \equiv (2n+1)J_n(x_s).
\end{equation}
Rearranging (\ref{eq:steadystatesolutions}) and multiplying by $P_n(x)$:
\begin{equation}\label{rearrange1}
T_nP_n = \frac{QH_n - \delta_{0n}A}{L_n}P_n(x)
\end{equation}
\begin{equation}\label{eq:takesum}
\implies T(x) = \sum_{n\textrm{ even}} T_nP_n(x) = \sum_{n\textrm{ even}}\frac{QH_n - \delta_{0n}A}{L_n}P_n(x) = \sum_{n\textrm{ even}}\frac{QH_nP_n(x)}{L_n} - \frac{A}{B}.
\end{equation}

\noindent
Truncating at $n=4$:
\begin{align*}\label{eq:truncate}
T(x) &= Q\left( \frac{H_0P_0(x)}{L_0} + \frac{H_2P_2(x)}{L_2} + \frac{H_4P_4(x)}{L_4}\right) - \frac{A}{B} \\
&= Q\left(\frac{J_0}{B} + \frac{5J_2P_2(x)}{6D+B} + \frac{9J_4P_4}{20D+B}\right) - \frac{A}{B}
\end{align*}
Evaluating at $x=x_s$:
\begin{equation*}
T_s = Q \frac{J_0(6D+B)(20D+B) + 5J_2P_2B(20D+B) + 9J_4P_4B(6D+B)}{B(6D+B)(20D+B)} - \frac{A}{B}
\end{equation*}
where $P_m = P_m(x_s)$ and $J_m = J_m(x_s)$ is implied. Rearranging gives
\begin{equation*}
\frac{A+BT_s}{Q}(20D+B)(6D+B) = J_0(6D+B)(20D+B) + 5J_2P_2B(20D+B) + 9J_4P_4B(6D+B),
\end{equation*}
which is a quadratic in $D$. Using $(20D+B)(6D+B) \equiv 120D^2 + 26BD + B^2$ and collecting terms with common factors of $D^2$, $D$ and $D^0$:
\begin{align*}
120\left( \frac{A+BT_s}{Q} - J_0 \right) D^2 &+ \left( \frac{26B(A+BT_s)}{Q} - 26BJ_0 - 100BJ_2P_2 - 54BJ_4P_4 \right) D + ... \\
... &+ \left( \frac{B^2(A+BT_s)}{Q} - B^2J_0 - 5B^2J_2P_2 - 9B^2J_4P_4 \right) = 0
\end{align*}

\clearpage
\noindent
This gives the solution for $D(x_s)$ as
\begin{equation}\label{eq:solution}
D(x_s) = \frac{- \beta \pm \sqrt{\beta^2 - 4\alpha \gamma}}{2\alpha},
\end{equation}
where
\begin{align*}
&\alpha = 120\left( \frac{A+BT_s}{Q} - J_0 \right) \\
&\beta = 2B\left( 13\left( \frac{A+BT_s}{Q} - J_0\right)  - 50J_2P_2 - 27J_4P_4 \right) \\
&\gamma = B^2\left( \frac{A+BT_s}{Q} - J_0 - 5J_2P_2 - 9J_4P_4 \right).
\end{align*}

%\vspace{5mm}
%\large
%\textbf{Physical solutions - conditions}
%\normalsize
%\vspace{5mm}

%We require $D>0$, or
%\begin{equation}\label{eq:condition1}
%\frac{-\beta \pm \sqrt{\beta^2 -4\alpha \gamma}}{2\alpha} > 0
%\end{equation}


\end{document}